Explicit namespaces for counter, lock and spawn.

heap_lang/lib/lock.v
@@ -3,6 +3,8 @@ From iris.proofmode Require Import invariants ghost_ownership.
 From iris.heap_lang Require Import proofmode notation.
 Import uPred.
 
+Definition lockN : namespace := nroot .@ "lock".
+
 Definition newlock : val := λ: <>, ref #false.
 Definition acquire : val :=
   rec: "acquire" "l" :=
@@ -25,11 +27,10 @@ Definition lock_inv (γ : gname) (l : loc) (R : iProp) : iProp :=
   (∃ b : bool, l ↦ #b ★ if b then True else own γ (Excl ()) ★ R)%I.
 
 Definition is_lock (l : loc) (R : iProp) : iProp :=
-  (∃ N γ, heapN ⊥ N ∧ heap_ctx ∧ inv N (lock_inv γ l R))%I.
+  (∃ γ, heap_ctx ∧ inv lockN (lock_inv γ l R))%I.
 
 Definition locked (l : loc) (R : iProp) : iProp :=
-  (∃ N γ, heapN ⊥ N ∧ heap_ctx ∧
-          inv N (lock_inv γ l R) ∧ own γ (Excl ()))%I.
+  (∃ γ, heap_ctx ∧ inv lockN (lock_inv γ l R) ∧ own γ (Excl ()))%I.
 
 Global Instance lock_inv_ne n γ l : Proper (dist n ==> dist n) (lock_inv γ l).
 Proof. solve_proper. Qed.
@@ -43,39 +44,38 @@ Global Instance is_lock_persistent l R : PersistentP (is_lock l R).
 Proof. apply _. Qed.
 
 Lemma locked_is_lock l R : locked l R ⊢ is_lock l R.
-Proof. rewrite /is_lock. iDestruct 1 as (N γ) "(?&?&?&_)"; eauto. Qed.
+Proof. rewrite /is_lock. iDestruct 1 as (γ) "(?&?&_)"; eauto. Qed.
 
-Lemma newlock_spec N (R : iProp) Φ :
-  heapN ⊥ N →
+Lemma newlock_spec (R : iProp) Φ :
   heap_ctx ★ R ★ (∀ l, is_lock l R -★ Φ #l) ⊢ WP newlock #() {{ Φ }}.
 Proof.
-  iIntros (?) "(#Hh & HR & HΦ)". rewrite /newlock.
+  iIntros "(#Hh & HR & HΦ)". rewrite /newlock.
   wp_seq. wp_alloc l as "Hl".
   iPvs (own_alloc (Excl ())) as (γ) "Hγ"; first done.
-  iPvs (inv_alloc N _ (lock_inv γ l R) with "[-HΦ]") as "#?"; first done.
+  iPvs (inv_alloc lockN _ (lock_inv γ l R) with "[-HΦ]") as "#?"; first done.
   { iIntros ">". iExists false. by iFrame. }
-  iPvsIntro. iApply "HΦ". iExists N, γ; eauto.
+  iPvsIntro. iApply "HΦ". iExists γ; eauto.
 Qed.
 
 Lemma acquire_spec l R (Φ : val → iProp) :
   is_lock l R ★ (locked l R -★ R -★ Φ #()) ⊢ WP acquire #l {{ Φ }}.
 Proof.
-  iIntros "[Hl HΦ]". iDestruct "Hl" as (N γ) "(%&#?&#?)".
+  iIntros "[Hl HΦ]". iDestruct "Hl" as (γ) "[#Hh #?]".
   iLöb as "IH". wp_rec. wp_focus (CAS _ _ _)%E.
-  iInv N as ([]) "[Hl HR]".
+  iInv lockN as ([]) "[Hl HR]".
   - wp_cas_fail. iPvsIntro; iSplitL "Hl".
     + iNext. iExists true; eauto.
     + wp_if. by iApply "IH".
   - wp_cas_suc. iPvsIntro. iDestruct "HR" as "[Hγ HR]". iSplitL "Hl".
     + iNext. iExists true; eauto.
-    + wp_if. iApply ("HΦ" with "[-HR] HR"). iExists N, γ; eauto.
+    + wp_if. iApply ("HΦ" with "[-HR] HR"). iExists γ; eauto.
 Qed.
 
 Lemma release_spec R l (Φ : val → iProp) :
   locked l R ★ R ★ Φ #() ⊢ WP release #l {{ Φ }}.
 Proof.
-  iIntros "(Hl&HR&HΦ)"; iDestruct "Hl" as (N γ) "(% & #? & #? & Hγ)".
-  rewrite /release. wp_let. iInv N as (b) "[Hl _]".
+  iIntros "(Hl&HR&HΦ)"; iDestruct "Hl" as (γ) "(#Hh & #? & Hγ)".
+  rewrite /release. wp_let. iInv lockN as (b) "[Hl _]".
   wp_store. iPvsIntro. iFrame "HΦ". iNext. iExists false. by iFrame.
 Qed.
 End proof.
