heap_lang/lib/spawn.v
@@ -3,6 +3,8 @@ From iris.proofmode Require Import invariants ghost_ownership.
 From iris.heap_lang Require Import proofmode notation.
 Import uPred.
 
+Definition spawnN : namespace := nroot .@ "spawn".
+
 Definition spawn : val :=
   λ: "f",
     let: "c" := ref NONE in
@@ -28,7 +30,7 @@ Proof. destruct H as (?&?). split. apply: inGF_inG. Qed.
 
 (** Now we come to the Iris part of the proof. *)
 Section proof.
-Context `{!heapG Σ, !spawnG Σ} (N : namespace).
+Context `{!heapG Σ, !spawnG Σ}.
 Local Notation iProp := (iPropG heap_lang Σ).
 
 Definition spawn_inv (γ : gname) (l : loc) (Ψ : val → iProp) : iProp :=
@@ -36,8 +38,7 @@ Definition spawn_inv (γ : gname) (l : loc) (Ψ : val → iProp) : iProp :=
                    ∃ v, lv = SOMEV v ★ (Ψ v ∨ own γ (Excl ()))))%I.
 
 Definition join_handle (l : loc) (Ψ : val → iProp) : iProp :=
-  (heapN ⊥ N ★ ∃ γ, heap_ctx ★ own γ (Excl ()) ★
-                    inv N (spawn_inv γ l Ψ))%I.
+  (∃ γ, heap_ctx ★ own γ (Excl ()) ★ inv spawnN (spawn_inv γ l Ψ))%I.
 
 Typeclasses Opaque join_handle.
 
@@ -51,19 +52,18 @@ Proof. solve_proper. Qed.
 (** The main proofs. *)
 Lemma spawn_spec (Ψ : val → iProp) e (f : val) (Φ : val → iProp) :
   to_val e = Some f →
-  heapN ⊥ N →
   heap_ctx ★ WP f #() {{ Ψ }} ★ (∀ l, join_handle l Ψ -★ Φ #l)
   ⊢ WP spawn e {{ Φ }}.
 Proof.
-  iIntros (<-%of_to_val ?) "(#Hh & Hf & HΦ)". rewrite /spawn.
+  iIntros (<-%of_to_val) "(#Hh & Hf & HΦ)". rewrite /spawn.
   wp_let. wp_alloc l as "Hl". wp_let.
   iPvs (own_alloc (Excl ())) as (γ) "Hγ"; first done.
-  iPvs (inv_alloc N _ (spawn_inv γ l Ψ) with "[Hl]") as "#?"; first done.
+  iPvs (inv_alloc spawnN _ (spawn_inv γ l Ψ) with "[Hl]") as "#?"; first done.
   { iNext. iExists NONEV. iFrame; eauto. }
   wp_apply wp_fork. iSplitR "Hf".
   - iPvsIntro. wp_seq. iPvsIntro. iApply "HΦ". rewrite /join_handle. eauto.
   - wp_focus (f _). iApply wp_wand_l. iFrame "Hf"; iIntros (v) "Hv".
-    iInv N as (v') "[Hl _]".
+    iInv spawnN as (v') "[Hl _]".
     wp_store. iPvsIntro. iSplit; [iNext|done].
     iExists (SOMEV v). iFrame. eauto.
 Qed.
@@ -71,8 +71,8 @@ Qed.
 Lemma join_spec (Ψ : val → iProp) l (Φ : val → iProp) :
   join_handle l Ψ ★ (∀ v, Ψ v -★ Φ v) ⊢ WP join #l {{ Φ }}.
 Proof.
-  rewrite /join_handle; iIntros "[[% H] Hv]". iDestruct "H" as (γ) "(#?&Hγ&#?)".
-  iLöb as "IH". wp_rec. wp_focus (! _)%E. iInv N as (v) "[Hl Hinv]".
+  rewrite /join_handle; iIntros "[H Hv]". iDestruct "H" as (γ) "(#?&Hγ&#?)".
+  iLöb as "IH". wp_rec. wp_focus (! _)%E. iInv spawnN as (v) "[Hl Hinv]".
   wp_load. iDestruct "Hinv" as "[%|Hinv]"; subst.
   - iPvsIntro; iSplitL "Hl"; [iNext; iExists _; iFrame; eauto|].
     wp_match. iApply ("IH" with "Hγ Hv").
