heap_lang/lib/par.v
@@ -12,16 +12,16 @@ Notation "e1 || e2" := (par (Pair (λ: <>, e1) (λ: <>, e2)))%E : expr_scope.
 Global Opaque par.
 
 Section proof.
-Context `{!heapG Σ, !spawnG Σ} (N : namespace).
+Context `{!heapG Σ, !spawnG Σ}.
 Local Notation iProp := (iPropG heap_lang Σ).
 
 Lemma par_spec (Ψ1 Ψ2 : val → iProp) e (f1 f2 : val) (Φ : val → iProp) :
-  heapN ⊥ N → to_val e = Some (f1,f2)%V →
+  to_val e = Some (f1,f2)%V →
   (heap_ctx ★ WP f1 #() {{ Ψ1 }} ★ WP f2 #() {{ Ψ2 }} ★
    ∀ v1 v2, Ψ1 v1 ★ Ψ2 v2 -★ ▷ Φ (v1,v2)%V)
   ⊢ WP par e {{ Φ }}.
 Proof.
-  iIntros (??) "(#Hh&Hf1&Hf2&HΦ)".
+  iIntros (?) "(#Hh&Hf1&Hf2&HΦ)".
   rewrite /par. wp_value. iPvsIntro. wp_let. wp_proj.
   wp_apply spawn_spec; try wp_done. iFrame "Hf1 Hh".
   iIntros (l) "Hl". wp_let. wp_proj. wp_focus (f2 _).
@@ -32,12 +32,11 @@ Qed.
 
 Lemma wp_par (Ψ1 Ψ2 : val → iProp)
     (e1 e2 : expr) `{!Closed [] e1, Closed [] e2} (Φ : val → iProp) :
-  heapN ⊥ N →
   (heap_ctx ★ WP e1 {{ Ψ1 }} ★ WP e2 {{ Ψ2 }} ★
    ∀ v1 v2, Ψ1 v1 ★ Ψ2 v2 -★ ▷ Φ (v1,v2)%V)
   ⊢ WP e1 || e2 {{ Φ }}.
 Proof.
-  iIntros (?) "(#Hh&H1&H2&H)". iApply (par_spec Ψ1 Ψ2); try wp_done.
+  iIntros "(#Hh&H1&H2&H)". iApply (par_spec Ψ1 Ψ2); try wp_done.
   iFrame "Hh H". iSplitL "H1"; by wp_let.
 Qed.
 End proof.
