tests/joining_existentials.v
@@ -77,8 +77,7 @@ Proof.
   wp_apply (newbarrier_spec N (barrier_res γ Φ)); auto.
   iFrame "Hh". iIntros (l) "[Hr Hs]".
   set (workers_post (v : val) := (barrier_res γ Ψ1 ★ barrier_res γ Ψ2)%I).
-  wp_let. wp_apply (wp_par _ (λ _, True)%I workers_post);
-    try iFrame "Hh"; first done.
+  wp_let. wp_apply (wp_par  (λ _, True)%I workers_post); iFrame "Hh".
   iSplitL "HP Hs Hγ"; [|iSplitL "Hr"].
   - wp_focus eM. iApply wp_wand_l; iSplitR "HP"; [|by iApply "He"].
     iIntros (v) "HP"; iDestruct "HP" as (x) "HP". wp_let.
@@ -88,8 +87,8 @@ Proof.
     iExists x; auto.
   - iDestruct (recv_weaken with "[] Hr") as "Hr"; first by iApply P_res_split.
     iPvs (recv_split with "Hr") as "[H1 H2]"; first done.
-    wp_apply (wp_par _ (λ _, barrier_res γ Ψ1)%I
-      (λ _, barrier_res γ Ψ2)%I); try iFrame "Hh"; first done.
+    wp_apply (wp_par (λ _, barrier_res γ Ψ1)%I
+                     (λ _, barrier_res γ Ψ2)%I); iFrame "Hh".
     iSplitL "H1"; [|iSplitL "H2"].
     + iApply worker_spec; auto.
     + iApply worker_spec; auto.
